Leaf count bound of the tree.

specs/Spec.Tree.fst
@@ -1,67 +1,152 @@
 module Spec.Tree
 
-open Lib.Rational
-open FStar.Mul
+module Math = FStar.Math.Lemmas
 
-type tree =
-  | Root: freq: pos -> left: tree -> right: tree -> tree
-  | Internal: freq: pos -> len: pos -> left: tree -> right: tree -> tree
-  | Leaf: freq: pos -> len: pos -> symbol: nat -> tree
+#set-options "--z3rlimit 200 --fuel 1 --ifuel 1"
+let height_one t =
+  if Leaf? t then
+    assert_norm(height t == 0)
+  else
+    if Leaf? (left t) then
+      if Leaf? (right t) then
+        ()
+      else
+        assert_norm(height (right t) >= 1)
+    else
+      assert_norm(height (left t) >= 1)
 
-let get_freq (t: tree{Root? t == false}): pos =
+let height_gt_one t =
   match t with
-  | Internal freq _ _ _ -> freq
-  | Leaf freq _ _ -> freq
+  | Root _ _ _ ->
+    if height (left t) < 1 then
+      assert_norm(height (right t) >= 1)
+    else
+      assert_norm(height (left t) >= 1)
+  | Internal _ _ _ _ ->
+    if height (left t) < 1 then
+      assert_norm(height (right t) >= 1)
+    else
+      assert_norm(height (left t) >= 1)
+  | Leaf _ _ _ -> ()
 
-let get_len (t: tree): nat =
-  match t with
-  | Root _ _ _ -> 0
-  | Internal _ len _ _ -> len
-  | Leaf _ len _ -> len
+#set-options "--z3rlimit 512 --fuel 2 --ifuel 2"
+let rec leaf_count_gt_height t h =
+  match height t with
+  | 0 -> ()
+  | 1 -> ()
+  | _ ->
+    assert_norm(
+      leaf_count t h == leaf_count (left t) (h - 1) + leaf_count (right t) (h - 1));
+    leaf_count_gt_height (left t) (h - 1);
+    leaf_count_gt_height (right t) (h - 1)
 
-let rec well_formed (t: tree): Type0 =
-  match t with
-  | Root f l r ->
-    Root? l == false /\ Root? r == false /\
-    get_len l == 1 /\ get_len r == 1 /\
-    well_formed l /\ well_formed r
-  | Internal f len l r ->
-    Root? l == false /\ Root? r == false /\
-    get_len l == len + 1 /\ get_len r == len + 1 /\
-    well_formed l /\ well_formed r
-  | _ -> True
+let rec do_total_leaf_count_gt_height (t: well_formed_tree) (h: pos): Lemma
+  (requires h >= height t)
+  (ensures do_total_leaf_count t h == do_total_leaf_count t (height t)) =
+  if h = height t + 1 || h = height t then
+    ()
+  else
+    calc (==) {
+      do_total_leaf_count t h;
+      =={}
+      do_total_leaf_count t (h - 1);
+      =={do_total_leaf_count_gt_height t (h - 1)}
+      do_total_leaf_count t (height t);
+    }
 
-private let rec optimal' (t: tree{well_formed t}): Type0 =
-  match t with
-  | Root f l r -> get_freq l + get_freq r == f /\ optimal' l /\ optimal' r
-  | Internal f len l r -> get_freq l + get_freq r == f /\ optimal' l /\ optimal' r
-  | Leaf _ _ _ -> True
+let rec do_total_leaf_count_lr (t: well_formed_tree) (h: pos): Lemma
+  (requires Leaf? t == false /\ 1 < h /\ h <= height t)
+  (ensures do_total_leaf_count t h ==
+    do_total_leaf_count (left t) (h - 1) + do_total_leaf_count (right t) (h - 1)) =
+  if h > 2 then
+    calc (==) {
+      do_total_leaf_count t h;
+      =={do_total_leaf_count_lr t (h - 1)}
+      leaf_count (left t) (h - 1) + leaf_count (right t) (h - 1) +
+      do_total_leaf_count (left t) (h - 2) + do_total_leaf_count (right t) (h - 2);
+      =={}
+      leaf_count (left t) (h - 1) + do_total_leaf_count (left t) (h - 2) +
+      leaf_count (right t) (h - 1) + do_total_leaf_count (right t) (h - 2);
+      =={
+        Math.paren_add_right 
+          (leaf_count (left t) (h - 1) + do_total_leaf_count (left t) (h - 2))
+          (leaf_count (right t) (h - 1))
+          (do_total_leaf_count (right t) (h - 2))
+      }
+      do_total_leaf_count (left t) (h - 1) + do_total_leaf_count (right t) (h - 1);
+    }
+  else
+    calc (==) {
+      do_total_leaf_count t 2;
+      =={}
+      leaf_count (left t) 1 + leaf_count (right t) 1 +
+      do_total_leaf_count t 1;
+      =={}
+      leaf_count (left t) 1 + leaf_count (right t) 1 +
+      leaf_count t 1 +
+      do_total_leaf_count t 0;
+      =={assert_norm(do_total_leaf_count t 0 == 0)}
+      leaf_count (left t) 1 + leaf_count (right t) 1 + leaf_count t 1;
+      =={}
+      leaf_count (left t) 1 + leaf_count (left t) 0 + 
+      leaf_count (right t) 1 + leaf_count (right t) 0;
+      =={
+        Math.paren_add_right
+          (leaf_count (left t) 1 + leaf_count (left t) 0)
+          (leaf_count (right t) 1)
+          (leaf_count (right t) 0)
+      }
+      leaf_count (left t) 1 + leaf_count (left t) 0 + 
+      (leaf_count (right t) 1 + leaf_count (right t) 0);
+      =={}
+      do_total_leaf_count (left t) 1 + do_total_leaf_count (right t) 1;
+    }
 
-let optimal (t: tree): Type0 = well_formed t /\ optimal' t
+let total_leaf_count_lr t =
+  match height t with
+  | 1 -> ()
+  | _ ->
+    calc (==) {
+      total_leaf_count t;
+      =={}
+      do_total_leaf_count t (height t);
+      =={do_total_leaf_count_lr t (height t)}
+      do_total_leaf_count (left t) (height t - 1) +
+      do_total_leaf_count (right t) (height t - 1);
+      =={
+        do_total_leaf_count_gt_height (left t) (height t - 1);
+        do_total_leaf_count_gt_height (right t) (height t - 1)
+      }
+      do_total_leaf_count (left t) (height (left t)) +
+      do_total_leaf_count (right t) (height (right t));
+      =={}
+      total_leaf_count (left t) + total_leaf_count (right t);
+    }
 
-type well_formed_tree = t: tree{well_formed t}
+let rec total_leaf_count_lower_bound t =
+  match height t with
+  | 0 -> ()
+  | 1 -> assert_norm(total_leaf_count t == 2)
+  | _ ->
+    total_leaf_count_lr t;
+    total_leaf_count_lower_bound (right t);
+    total_leaf_count_lower_bound (left t)
 
-unfold let kraft_term (n: nat): rat = (1, pow2 n)
-
-let kraft_term_plus (n: pos): Lemma
-  (ensures kraft_term n +$ kraft_term n =$ kraft_term (n - 1))
-  [SMTPat (kraft_term n +$ kraft_term n)] = ()
-
-let rec term_times (l: pos) (n: nat): rat =
-  match n with
-  | 0 -> zero
-  | _ -> kraft_term l +$ term_times l (n - 1)
-
-let rec kraft_sum (t: well_formed_tree): rat =
-  match t with
-  | Root _ l r -> kraft_sum l +$ kraft_sum r
-  | Internal _ _ l r -> kraft_sum l +$ kraft_sum r
-  | Leaf _ len _ -> kraft_term len
+let rec total_leaf_count_upper_bound t =
+  match height t with
+  | 0 -> ()
+  | 1 -> assert_norm(total_leaf_count t == pow2 1)
+  | _ ->
+    total_leaf_count_lr t;
+    total_leaf_count_upper_bound (right t);
+    total_leaf_count_upper_bound (left t);
+    if height (left t) < height (right t) then
+      Math.pow2_le_compat (height t - 1) (height (left t))
+    else
+      Math.pow2_le_compat (height t - 1) (height (right t))
 
 #set-options "--z3rlimit 200"
-let rec kraft_sum_non_root (t: well_formed_tree): Lemma
-  (requires Root? t == false)
-  (ensures kraft_sum t =$ kraft_term (get_len t)) =
+let rec kraft_sum_non_root t =
   match t with
   | Internal _ len l r ->
     calc (=$) {
@@ -83,3 +168,9 @@ let rec kraft_sum_non_root (t: well_formed_tree): Lemma
       kraft_term len;
     }
   | Leaf _ len _ -> ()
+
+let kraft_sum_root t =
+  match t with
+  | Root _ l r ->
+    kraft_sum_non_root l;
+    kraft_sum_non_root r
