code/Yazi.Tree.Types.fsti
@@ -1,0 +1,90 @@
+module Yazi.Tree.Types
+
+module B = LowStar.Buffer
+module CB = LowStar.ConstBuffer
+module U16 = FStar.UInt16
+module U32 = FStar.UInt32
+module U8 = FStar.UInt8
+
+open Yazi.Deflate.Constants
+
+noeq
+type ct_data = {
+  freq_or_dad: U16.t;
+  code_or_len: U16.t;
+}
+
+type dyn_ltree_t = tree: B.buffer ct_data{
+  B.len tree == heap_size
+}
+
+type dyn_dtree_t = tree: B.buffer ct_data{
+  let open U32 in
+  B.length tree == U32.v (2ul *^ d_codes +^ 1ul)
+}
+
+type bl_tree_t = tree: B.buffer ct_data{
+  let open U32 in
+  B.len tree == 2ul *^ bl_codes +^ 1ul
+}
+
+noeq
+type static_tree_desc = {
+  static_tree: CB.const_buffer ct_data;
+  extra_bits: CB.const_buffer U32.t;
+  extra_base: U32.t;
+  elems: U32.t;
+  max_length: U32.t;
+}
+
+noeq
+type tree_desc = {
+  max_code: U32.t;
+  stat_desc: CB.const_buffer static_tree_desc;
+}
+
+type bl_count_t = count: B.buffer U16.t{
+  let open U32 in
+  B.len count == max_bits +^ 1ul
+}
+
+type tree_heap_t = heap: B.buffer U32.t{
+  let open U32 in
+  B.len heap == 2ul *^ l_codes +^ 1ul
+}
+
+type tree_depth_t = depth: B.buffer U8.t{
+  let open U32 in
+  B.len depth == 2ul *^ l_codes +^ 1ul
+}
+
+type lit_bufsize_t = s: U32.t {
+  let open U32 in
+  v s == pow2 7 \/ v s == pow2 8 \/
+  v s == pow2 9 \/ v s == pow2 10 \/
+  v s == pow2 11 \/ v s == pow2 12 \/
+  v s == pow2 13 \/ v s == pow2 14 \/
+  v s == pow2 15 \/ v s == pow2 16
+}
+
+noeq
+type tree_context = {
+  dyn_ltree: dyn_ltree_t;
+  dyn_dtree: dyn_dtree_t;
+  bl_tree: dyn_ltree_t;
+
+  l_desc: tree_desc;
+  d_desc: tree_desc;
+  bl_desc: tree_desc;
+
+  bl_count: bl_count_t;
+  heap: tree_heap_t;
+  depth: tree_depth_t;
+
+  l_buf: B.buffer U8.t;
+  d_buf: B.buffer U8.t;
+  pending_buf: B.buffer U8.t;
+
+  lit_bufsize: lit_bufsize_t;
+  pending_buf_size: U32.t;
+}
