specs/Spec.Tree.fsti
@@ -1,0 +1,226 @@
+module Spec.Tree
+
+module B = LowStar.Buffer
+module CB = LowStar.ConstBuffer
+module HS = FStar.HyperStack
+module U32 = FStar.UInt32
+
+open Lib.Rational
+open Lib.Seq
+open FStar.Mul
+open FStar.Seq
+open Yazi.Tree.Types
+
+type tree =
+  | Root: freq: pos -> left: tree -> right: tree -> tree
+  | Internal: freq: pos -> len: pos -> left: tree -> right: tree -> tree
+  | Leaf: freq: pos -> len: pos -> symbol: nat -> tree
+
+let freq (t: tree{Root? t == false}): pos =
+  match t with
+  | Internal freq _ _ _ -> freq
+  | Leaf freq _ _ -> freq
+
+let length (t: tree): nat =
+  match t with
+  | Root _ _ _ -> 0
+  | Internal _ len _ _ -> len
+  | Leaf _ len _ -> len
+
+let rec well_formed (t: tree): Type0 =
+  match t with
+  | Root f l r ->
+    Root? l == false /\ Root? r == false /\
+    length l == 1 /\ length r == 1 /\
+    well_formed l /\ well_formed r
+  | Internal f len l r ->
+    Root? l == false /\ Root? r == false /\
+    length l == len + 1 /\ length r == len + 1 /\
+    well_formed l /\ well_formed r
+  | _ -> True
+
+private let rec optimal' (t: tree{well_formed t}): Type0 =
+  match t with
+  | Root f l r -> freq l + freq r == f /\ optimal' l /\ optimal' r
+  | Internal f len l r -> freq l + freq r == f /\ optimal' l /\ optimal' r
+  | Leaf _ _ _ -> True
+
+let optimal (t: tree): Type0 = well_formed t /\ optimal' t
+
+type well_formed_tree = t: tree{well_formed t}
+
+type root = t: well_formed_tree{Root? t == true}
+
+type internal = t: well_formed_tree{Internal? t == true}
+
+type leaf = t: well_formed_tree{Leaf? t == true}
+
+type non_leaf = t: well_formed_tree{Leaf? t == false}
+
+let left (t: non_leaf): well_formed_tree =
+  match t with
+  | Root _ l _ -> l
+  | Internal _ _ l _ -> l
+
+let right (t: non_leaf): well_formed_tree =
+  match t with
+  | Root _ _ r -> r
+  | Internal _ _ _ r -> r
+
+let rec height (t: well_formed_tree): Tot nat =
+  match t with
+  | Root _ l r ->
+    let ld = height l in
+    let rd = height r in
+    1 + (if ld > rd then ld else rd)
+  | Internal _ _ l r ->
+    let ld = height l in
+    let rd = height r in
+    1 + (if ld > rd then ld else rd)
+  | Leaf _ len _ -> 0
+
+let rec leaf_count (t: well_formed_tree) (h: nat): Tot nat =
+  match t with
+  | Root _ l r -> 
+    if h > 0 then leaf_count l (h - 1) + leaf_count r (h - 1) else 0
+  | Internal _ _ l r ->
+    if h > 0 then leaf_count l (h - 1) + leaf_count r (h - 1) else 0
+  | Leaf _ len' _ ->
+    if h = 0 then 1 else 0
+
+private let rec do_total_leaf_count (t: well_formed_tree) (h: nat): Tot nat =
+  leaf_count t h + (if h > 0 then do_total_leaf_count t (h - 1) else 0)
+
+let total_leaf_count (t: well_formed_tree) = do_total_leaf_count t (height t)
+
+val height_one: (t: well_formed_tree) -> Lemma
+  (requires height t  == 1)
+  (ensures Leaf? t == false /\ Leaf? (left t) /\ Leaf? (right t))
+  [SMTPat (height t)]
+
+val height_gt_one: (t: well_formed_tree) -> Lemma
+  (requires height t > 1)
+  (ensures Leaf? t == false /\ (Leaf? (left t) == false \/ Leaf? (right t) == false))
+  [SMTPat (height t)]
+
+val leaf_count_gt_height: (t: well_formed_tree) -> (h: nat{h > height t}) -> Lemma
+  (ensures leaf_count t h == 0)
+  [SMTPat (leaf_count t h)]
+
+val total_leaf_count_lr: (t: non_leaf) -> Lemma
+  (ensures total_leaf_count t = total_leaf_count (left t) + total_leaf_count (right t))
+  [SMTPat (total_leaf_count t)]
+
+val total_leaf_count_lower_bound: (t: well_formed_tree) -> Lemma
+  (ensures total_leaf_count t >= 1 + height t)
+  [SMTPat (total_leaf_count t)]
+
+val total_leaf_count_upper_bound: (t: well_formed_tree) -> Lemma
+  (ensures total_leaf_count t <= pow2 (height t))
+  [SMTPat (total_leaf_count t)]
+
+private let rec do_leaf_count_seq
+  (t: root)
+  (h: nat{h <= height t}) :
+  s: Seq.seq nat{
+    Seq.length s == h + 1 /\ (forall i. {:pattern (s.[i])} s.[i] == leaf_count t i)
+  } =
+  if h > 0 then
+    do_leaf_count_seq t (h - 1) `snoc` leaf_count t h
+  else
+    Seq.create 1 (leaf_count t h)
+
+type lc_seq (t: root) = s: Seq.seq nat{
+  Seq.length s == height t + 1 /\ (forall i. {:pattern (s.[i])} s.[i] == leaf_count t i)
+}
+  
+let leaf_count_seq (t: root): lc_seq t =
+  do_leaf_count_seq t (height t)
+
+unfold let kraft_term (n: nat): rat = (1, pow2 n)
+
+let kraft_term_plus (n: pos): Lemma
+  (ensures kraft_term n +$ kraft_term n =$ kraft_term (n - 1))
+  [SMTPat (kraft_term n +$ kraft_term n)] = ()
+
+let rec term_times (l: pos) (n: nat): rat =
+  match n with
+  | 0 -> zero
+  | _ -> kraft_term l +$ term_times l (n - 1)
+
+let rec kraft_sum (t: well_formed_tree): rat =
+  match t with
+  | Root _ l r -> kraft_sum l +$ kraft_sum r
+  | Internal _ _ l r -> kraft_sum l +$ kraft_sum r
+  | Leaf _ len _ -> kraft_term len  
+
+#set-options "--z3rlimit 200"
+val kraft_sum_non_root: (t: well_formed_tree) -> Lemma
+  (requires Root? t == false)
+  (ensures kraft_sum t =$ kraft_term (length t))
+  [SMTPat (kraft_sum t)]
+
+val kraft_sum_root: (t: well_formed_tree) -> Lemma
+  (requires Root? t == true)
+  (ensures kraft_sum t =$ one)
+  [SMTPat (kraft_sum t)]
+
+let rec kraft_sum_seq (s: Seq.seq nat) (base i: nat): 
+  Tot rat
+  (decreases (Seq.length s - i)) =
+  if i < Seq.length s then
+    (s.[i], pow2 (i + base)) +$ kraft_sum_seq s base (i + 1)
+  else
+    zero
+
+let tree_context_valid (h: HS.mem) (c: CB.const_buffer tree_context) =
+  CB.length c == 1 /\ CB.live h c /\
+  (let ctx = B.get h (CB.as_mbuf c) 0 in
+  B.live h ctx.dyn_ltree /\ B.live h ctx.dyn_dtree /\ B.live h ctx.bl_tree /\
+  B.live h ctx.bl_count /\ B.live h ctx.heap /\ B.live h ctx.depth /\ B.live h ctx.l_buf /\
+  B.live h ctx.d_buf /\ B.live h ctx.pending_buf /\
+  CB.live h ctx.l_desc.stat_desc /\ CB.live h ctx.d_desc.stat_desc /\
+  CB.live h ctx.bl_desc.stat_desc /\
+
+  B.frameOf ctx.dyn_dtree == B.frameOf ctx.dyn_ltree /\
+  B.frameOf ctx.bl_tree == B.frameOf ctx.dyn_ltree /\
+  B.frameOf ctx.bl_count == B.frameOf ctx.dyn_ltree /\
+  B.frameOf ctx.heap == B.frameOf ctx.dyn_ltree /\
+  B.frameOf ctx.depth == B.frameOf ctx.dyn_ltree /\
+  B.frameOf ctx.l_buf == B.frameOf ctx.dyn_ltree /\
+  B.frameOf ctx.d_buf == B.frameOf ctx.dyn_ltree /\
+  B.frameOf ctx.pending_buf == B.frameOf ctx.dyn_ltree /\
+
+  B.frameOf (CB.as_mbuf ctx.l_desc.stat_desc) ==
+  B.frameOf (CB.as_mbuf ctx.d_desc.stat_desc) /\
+  B.frameOf (CB.as_mbuf ctx.bl_desc.stat_desc) ==
+  B.frameOf (CB.as_mbuf ctx.d_desc.stat_desc) /\
+
+  HS.disjoint (B.frameOf (CB.as_mbuf ctx.d_desc.stat_desc)) (B.frameOf ctx.dyn_ltree) /\
+  
+  B.disjoint ctx.dyn_ltree ctx.dyn_dtree /\ B.disjoint ctx.dyn_ltree ctx.bl_tree /\
+  B.disjoint ctx.dyn_ltree ctx.bl_count /\ B.disjoint ctx.dyn_ltree ctx.heap /\
+  B.disjoint ctx.dyn_ltree ctx.depth /\ B.disjoint ctx.dyn_ltree ctx.l_buf /\
+  B.disjoint ctx.dyn_ltree ctx.d_buf /\ B.disjoint ctx.dyn_ltree ctx.pending_buf /\
+  B.disjoint ctx.dyn_dtree ctx.bl_tree /\ B.disjoint ctx.dyn_dtree ctx.bl_count /\
+  B.disjoint ctx.dyn_dtree ctx.heap /\ B.disjoint ctx.dyn_dtree ctx.depth /\
+  B.disjoint ctx.dyn_dtree ctx.l_buf /\ B.disjoint ctx.dyn_dtree ctx.d_buf /\
+  B.disjoint ctx.dyn_dtree ctx.pending_buf /\ B.disjoint ctx.bl_tree ctx.bl_count /\
+  B.disjoint ctx.bl_tree ctx.heap /\ B.disjoint ctx.bl_tree ctx.depth /\
+  B.disjoint ctx.bl_tree ctx.l_buf /\ B.disjoint ctx.bl_tree ctx.d_buf /\
+  B.disjoint ctx.bl_tree ctx.pending_buf /\ B.disjoint ctx.bl_count ctx.heap /\
+  B.disjoint ctx.bl_count ctx.depth /\ B.disjoint ctx.bl_count ctx.l_buf /\
+  B.disjoint ctx.bl_count ctx.d_buf /\ B.disjoint ctx.bl_count ctx.pending_buf /\
+  B.disjoint ctx.heap ctx.depth /\ B.disjoint ctx.heap ctx.l_buf /\
+  B.disjoint ctx.heap ctx.d_buf /\ B.disjoint ctx.heap ctx.pending_buf /\ 
+  B.disjoint ctx.depth ctx.l_buf /\ B.disjoint ctx.depth ctx.d_buf /\
+  B.disjoint ctx.depth ctx.pending_buf /\ B.disjoint ctx.l_buf ctx.d_buf /\
+  B.disjoint ctx.l_buf ctx.pending_buf /\ B.disjoint ctx.d_buf ctx.pending_buf /\
+  
+  4 * U32.v ctx.lit_bufsize == U32.v ctx.pending_buf_size /\
+  B.length ctx.l_buf == U32.v ctx.lit_bufsize /\
+  B.length ctx.d_buf == U32.v ctx.lit_bufsize /\
+  B.length ctx.pending_buf == U32.v ctx.pending_buf_size /\
+  CB.length ctx.l_desc.stat_desc == 1 /\
+  CB.length ctx.d_desc.stat_desc == 1 /\
+  CB.length ctx.bl_desc.stat_desc == 1)
